rough cut of LR

theories/iris/logrel.v
@@ -256,70 +256,21 @@ Section instr.
     | SWords ws => n = length ws
     end.
 
-  Definition svalue_in_skind (sv : semantic_value) (sκ : skind) : Prop :=
-    match sκ with
-    | SVALTYPE ιs ξ => has_areps ιs sv /\ ref_flag_atoms_interp ξ sv
-    | SMEMTYPE n ξ => ssize_interp n sv /\ ref_flag_words_interp ξ sv
-    end.
+  Program Definition svalue_in_skind : leibnizO skind -n> leibnizO semantic_value -n> PropO :=
+    λne sκ sv,
+      match sκ with
+      | SVALTYPE ιs ξ => has_areps ιs sv /\ ref_flag_atoms_interp ξ sv
+      | SMEMTYPE n ξ => ssize_interp n sv /\ ref_flag_words_interp ξ sv
+      end.
 
   Definition stype_in_skind (T : SVR) (sκ : skind) : Prop :=
-    forall sv, T sv -∗ ⌜svalue_in_skind sv sκ⌝.
+    forall sv, T sv -∗ ⌜svalue_in_skind sκ sv⌝.
 
   (*
   Definition values_interp0 (vrel : value_relation) (se : semantic_env) :
     leibnizO (list type) -n> OsR :=
     λne τs os,
       (∃ oss, ⌜os = concat oss⌝ ∗ [∗ list] τ; os ∈ τs; oss, vrel τ se (SAtoms os))%I. *)
-
-  Definition type_skind (se : semantic_env) (τ : type) : option skind :=
-    match τ with
-    | VarT x => fst <$> lookup_type se x
-    | NumT κ _
-    | SumT κ _
-    | VariantT κ _
-    | ProdT κ _
-    | StructT κ _
-    | RefT κ _ _
-    | I31T κ
-    | CodeRefT κ _
-    | SerT κ _
-    | RecT κ _
-    | PlugT κ _
-    | SpanT κ _
-    | ExistsMemT κ _
-    | ExistsRepT κ _
-    | ExistsSizeT κ _
-    | ExistsTypeT κ _ _ => eval_kind se κ
-    end.
-
-  Definition skind_rep (κ : skind) : option (list atomic_rep) :=
-    match κ with
-    | SVALTYPE ιs _ => Some ιs
-    | _ => None
-    end.
-
-  Definition type_arep (se : semantic_env) (τ : type) : option (list atomic_rep) :=
-    κ ← type_skind se τ;
-    skind_rep κ.
-
-  Definition translate_type (se : semantic_env) (τ : type) : option (list W.value_type) :=
-    map translate_arep <$> type_arep se τ.
-  
-  Definition translate_types (se : semantic_env) (τs : list type) : option (list W.value_type) :=
-    @concat _ <$> mapM (translate_type se) τs.
-
-  (* Value type interpretations. *)
-  Program Definition type_var_interp : leibnizO nat -n> SVRO :=
-    λne t se,
-      default (λne _, False%I) (snd <$> lookup_type se t).
-  Solve All Obligations with solve_proper.
-
-  Program Definition i31_interp : SVR :=
-    λne _, True%I.
-
-  Program Definition num_interp : leibnizO num_type -n> SVR :=
-    λne nt _, True%I.
-
   Program Definition eval_rep_se : semantic_env -n> leibnizO representation -n> leibnizO (option (list atomic_rep)) :=
     λne se ρ, eval_rep se ρ.
   Next Obligation.
@@ -343,6 +294,75 @@ Section instr.
       cbn; intros.
       by apply H1.
   Qed.
+
+  Program Definition eval_size_se : semantic_env -n> leibnizO size -n> leibnizO (option nat).
+  Admitted.
+
+  Program Definition eval_kind_se : semantic_env -n> leibnizO kind -n> leibnizO (option skind) :=
+    λne se κ, eval_kind se κ.
+  Next Obligation.
+    solve_proper.
+  Qed.
+  Next Obligation.
+  Admitted.
+
+  Program Definition type_skind : semantic_env -n> leibnizO type -n> leibnizO (option skind) :=
+    λne se τ,
+    match τ with
+    | VarT x => fst <$> lookup_type se x
+    | NumT κ _
+    | SumT κ _
+    | VariantT κ _
+    | ProdT κ _
+    | StructT κ _
+    | RefT κ _ _
+    | I31T κ
+    | CodeRefT κ _
+    | SerT κ _
+    | RecT κ _
+    | PlugT κ _
+    | SpanT κ _
+    | ExistsMemT κ _
+    | ExistsRepT κ _
+    | ExistsSizeT κ _
+    | ExistsTypeT κ _ _ => eval_kind_se se κ
+    end.
+  Next Obligation.
+    cbn.
+    repeat intros ?; cbn.
+    rewrite H.
+    solve_proper.
+  Qed.
+  Next Obligation.
+  Admitted.
+
+  Definition skind_rep (κ : skind) : option (list atomic_rep) :=
+    match κ with
+    | SVALTYPE ιs _ => Some ιs
+    | _ => None
+    end.
+
+  Definition type_arep (se : semantic_env) (τ : type) : option (list atomic_rep) :=
+    κ ← type_skind se τ;
+    skind_rep κ.
+
+  Definition translate_type (se : semantic_env) (τ : type) : option (list W.value_type) :=
+    map translate_arep <$> type_arep se τ.
+  
+  Definition translate_types (se : semantic_env) (τs : list type) : option (list W.value_type) :=
+    @concat _ <$> mapM (translate_type se) τs.
+
+  (* Value type interpretations. *)
+  Program Definition type_var_interp : leibnizO nat -n> SVRO :=
+    λne t se,
+      default (λne _, False%I) (snd <$> lookup_type se t).
+  Solve All Obligations with solve_proper.
+
+  Program Definition i31_interp : semantic_type :=
+    λne _ _, True%I.
+
+  Program Definition num_interp : leibnizO num_type -n> semantic_type :=
+    λne nt se _, True%I.
 
   Program Definition eval_mem_se : semantic_env -n> leibnizO memory -n> leibnizO (option base_memory) :=
     λne se ρ, eval_mem se ρ.
@@ -375,44 +395,29 @@ Section instr.
     eapply H.
   Qed.
 
-  Program Definition sum_interp (ρs : list representation) : listO SVRO -n> SVRO :=
-    λne (τs : list SVRO) (se : semantic_env) sv,
-      (∃ (i : nat) os off count,
-         ⌜sv = SAtoms (I32A (Wasm_int.int_of_Z i32m (Z.of_nat i)) :: os)⌝ ∗
-         ⌜sum_offset_se se ρs i = Some off⌝ ∗
-         ⌜length <$> ρs !! i ≫= eval_rep se = Some count⌝ ∗
-         match list_lookup i τs with
-         | Some τi => τi se (SAtoms (take count (drop off os)))
-         | None => False%I
-         end)%I.
-  Next Obligation.
-    solve_proper.
-  Qed.
-  Next Obligation.
-    intros ρs τs n se se' Hse sv.
-    cbn.
-    repeat (f_equiv;
-            try match goal with
-                | |- se = se' => fail 2
-                | |- eval_rep se = eval_rep se' => fail 2
-              end).
-    - by eapply sum_offset_se.
-    - destruct (ρs !! a); cbn; auto.
-      by eapply eval_rep_se.
-    - destruct (list_lookup a τs); solve_proper.
-  Qed.
-  Next Obligation.
-    intros * se se' Hse sv sv'.
-    cbn.
-    repeat f_equiv.
-    assert (Haa: se  !! a ≡{n}≡ se' !! a) by solve_proper.
-    inversion Haa as [τi τi' Haa' Ha Ha'|Ha Ha']; unfold lookup in *;
-      rewrite -Ha -Ha'.
-    - apply Haa'.
-    - done.
-  Qed.
+  Program Definition sum_interp κ : listO SVRO -> SVRO :=
+    match κ with
+    | VALTYPE (SumR ρs) _ =>
+        λne (τs : list SVRO) (se : semantic_env) sv,
+          ∃ (i : nat) os off count,
+            ⌜sv = SAtoms (I32A (Wasm_int.int_of_Z i32m (Z.of_nat i)) :: os)⌝ ∗
+            ⌜sum_offset_se se ρs i = Some off⌝ ∗
+            ⌜length <$> ρs !! i ≫= eval_rep se = Some count⌝ ∗
+            match list_lookup i τs with
+            | Some τi => τi se (SAtoms (take count (drop off os)))
+            | None => False%I
+            end
+    | _ => λne _ _ _, False
+    end%I.
+  Next Obligation. Admitted.
+  Next Obligation. Admitted.
+  Next Obligation. Admitted.
+  Next Obligation. Admitted.
+  Next Obligation. Admitted.
+  Next Obligation. Admitted.
+  Next Obligation. Admitted.
 
-  Program Definition variant_interp : list semantic_type -n> semantic_env -n> SVR :=
+  Program Definition variant_interp : list semantic_type -> semantic_env -n> SVR :=
     λne (τs : listO semantic_type) se sv,
       (∃ i n ws ws',
          ⌜N_nat_repr i n⌝ ∗
@@ -536,54 +541,10 @@ Section instr.
     solve_proper.
   Qed.
 
-  Program Fixpoint type_interp (τ : leibnizO type) : semantic_env -n> SVR :=
-      match τ with
-      | VarT t =>
-          type_var_interp t
-      | I31T _ => i31_interp
-      | NumT _ nt => num_interp nt
-      | SumT (VALTYPE (SumR ρs) _) τs =>
-          sum_interp ρs (map type_interp τs)
-      | SumT _ _ => λne _ _, False%I
-      | VariantT _ τs => variant_interp (map type_interp τs)
-      | ProdT _ τs => prod_interp (map type_interp τs)
-      | StructT _ τs => struct_interp (map type_interp τs)
-      | RefT _ μ τ => ref_interp μ (type_interp τ)
-      | _ => λne se (sv : leibnizO semantic_value), emp%I
-      end.
-
-  Fixpoint type_interp (τ : leibnizO type) : semantic_env -n> SVR :=
-    λne (se : semantic_env),
-      match τ with
-      | VarT t => type_var_interp se t
-      | I31T _ => i31_interp
-      | NumT _ nt => num_interp nt
-      | _ => λne (sv : leibnizO semantic_value), emp%I
-      end.
-      | SumT (VALTYPE (SumR ρs) _) τs => sum_interp ρs (map type_interp τs) se
-      | _ => λne _, False%I
-      end.
-      | SumT _ _ => λne _, False
-      | VariantT _ τs => variant_interp vrel se τs
-      | ProdT _ τs => prod_interp vrel se τs
-      | StructT _ τs => struct_interp vrel se τs
-      | RefT _ μ τ => ref_interp vrel se μ τ
-      | RefT _ (BaseM MemMM) τ => ref_mm_interp vrel se τ
-      | RefT _ (BaseM MemGC) τ => ref_gc_interp vrel se τ
-      | CodeRefT _ ϕ => coderef_interp vrel se ϕ
-      | SerT _ τ => ser_interp vrel se τ
-      | PlugT _ ρ => plug_interp se ρ
-      | SpanT _ σ => span_interp se σ
-      | RecT κ τ => rec_interp vrel se κ τ
-      | ExistsMemT _ τ => exists_mem_interp vrel se τ
-      | ExistsRepT _ τ => exists_rep_interp vrel se τ
-      | ExistsSizeT _ τ => exists_size_interp vrel se τ
-      | ExistsTypeT _ κ τ => exists_type_interp vrel se κ τ
-      end%I.
-
-  Definition mono_closure_interp0 vrel (se : semantic_env) :
-    leibnizO (list type) -n> leibnizO (list type) -n> ClR :=
-    λne τs1 τs2 cl,
+  Definition mono_closure_interp0 :
+    listO semantic_type -n> listO semantic_type -n> semantic_env -n> ClR.
+    Admitted.
+    (*λne τs1 τs2 cl,
       match cl with
       | FC_func_native inst (Tf ts1 ts2) tlocs es =>
           ⌜translate_types se τs1 = Some ts1⌝ ∗
@@ -601,196 +562,275 @@ Section instr.
             in
             CWP es UNDER [(length ts2, const Φ)]; Some (length ts2, Φ) {{ const Φ }}
       | FC_func_host _ _ => False
-      end%I.
+      end%I.*)
 
-  Fixpoint closure_interp0
-    (vrel : value_relation) (se : semantic_env) (ϕ : leibnizO function_type) : ClR :=
-    λne cl,
-      match ϕ with
-      | MonoFunT τs1 τs2 => mono_closure_interp0 vrel se τs1 τs2 cl
-      | ForallMemT ϕ' => ∀ μ, closure_interp0 vrel (senv_insert_mem μ se) ϕ' cl
-      | ForallRepT ϕ' => ∀ ιs, closure_interp0 vrel (senv_insert_rep ιs se) ϕ' cl
-      | ForallSizeT ϕ' => ∀ n, closure_interp0 vrel (senv_insert_size n se) ϕ' cl
-      | ForallTypeT κ ϕ' =>
-          ∃ sκ,
-            ⌜eval_kind se κ = Some sκ⌝ ∗
-              ∀ sκ_T T,
-                ⌜subskind_of sκ_T sκ⌝ -∗
-                ⌜stype_in_skind T sκ_T⌝ -∗
-                closure_interp0 vrel (senv_insert_type sκ_T T se) ϕ' cl
-      end%I.
-
-  (* TODO *)
-  Global Instance Persistent_closure_interp0 vrel se ϕ cl : Persistent (closure_interp0 vrel se ϕ cl).
-  Admitted.
-
-  Global Instance closure_interp0_ne vrel se ϕ : NonExpansive2 (closure_interp0 vrel se).
-  Admitted.
-
-  Definition variant_interp
-    (vrel : value_relation) (se : semantic_env) (τs : list type) : SVR :=
-    λne sv,
-      (∃ i n ws ws' τ,
-         ⌜N_nat_repr i n⌝ ∗
-         ⌜sv = SWords (WordInt n :: ws ++ ws')⌝ ∗
-         ⌜τs !! i = Some τ⌝ ∗
-         ▷ vrel se τ (SWords ws))%I.
-
-  Definition prod_interp (vrel : value_relation) (se : semantic_env) (τs : list type) : SVR :=
-    λne sv,
-      (∃ oss, ⌜sv = SAtoms (concat oss)⌝ ∗ [∗ list] τ; os ∈ τs; oss, vrel se τ (SAtoms os))%I.
-
-  Definition struct_interp (vrel : value_relation) (se : semantic_env) (τs : list type) : SVR :=
-    λne sv,
-      (∃ wss,
-         ⌜sv = SWords (concat wss)⌝ ∗ [∗ list] ws; τ ∈ wss; τs, vrel se τ (SWords ws))%I.
-
-  Definition ref_mm_interp (vrel : value_relation) : leibnizO semantic_env -n> leibnizO type -n> SVR :=
-    λne se τ sv,
-      (∃ ℓ fs ws,
-         ⌜sv = SAtoms [PtrA (PtrHeap MemMM ℓ)]⌝ ∗
-           ℓ ↦layout fs ∗
-           ℓ ↦heap ws ∗
-           ▷ vrel se τ (SWords ws))%I.
-
-  Definition ref_gc_interp (vrel : value_relation) : semantic_env -n> type -n> SVR :=
-    λne vrel se τ sv,
-      (∃ ℓ fs,
-         ⌜sv = SAtoms [PtrA (PtrHeap MemGC ℓ)]⌝ ∗
-           na_inv logrel_nais (ns_ref ℓ)
-             (∃ ws, ℓ ↦layout fs ∗ ℓ ↦heap ws ∗ ▷ vrel se τ (SWords ws)))%I.
-
-  Definition ref_interp : value_relation -n> semantic_env -n> leibnizO memory -n> leibnizO type -n> SVR :=
-    λne vrel se (μ : leibnizO memory),
-      match eval_mem se μ with
-      | Some MemMM => ref_mm_interp vrel se
-      | Some MemGC => ref_gc_interp vrel se
-      | None => False
-      end.
-
-  Definition coderef_interp (vrel : value_relation) (se : semantic_env) (ϕ : function_type) : SVR :=
-    λne sv,
+  Program Definition coderef_interp : (semantic_env -n> ClR) -n> semantic_type :=
+    λne FT se sv,
       (∃ i i32 j cl,
          ⌜N_i32_repr i i32⌝ ∗
-           ⌜sv = SAtoms [I32A i32]⌝ ∗
-           closure_interp0 vrel se ϕ cl ∗
-           na_inv logrel_nais (ns_tab i) (N.of_nat sr.(sr_table) ↦[wt][i] Some j) ∗
-           na_inv logrel_nais (ns_fun (N.of_nat j)) (N.of_nat j ↦[wf] cl))%I.
+         ⌜sv = SAtoms [I32A i32]⌝ ∗
+         FT se cl ∗
+         na_inv logrel_nais (ns_tab i) (N.of_nat sr.(sr_table) ↦[wt][i] Some j) ∗
+         na_inv logrel_nais (ns_fun (N.of_nat j)) (N.of_nat j ↦[wf] cl))%I.
+  Next Obligation. solve_proper. Qed.
+  Next Obligation. solve_proper. Qed.
+  Next Obligation. solve_proper. Qed.
 
-  Definition ser_interp (vrel : value_relation) (se : semantic_env) (τ : type) : SVR :=
-    λne sv,
-      (∃ os, ⌜sv = SWords (flat_map serialize_atom os)⌝ ∗ ▷ vrel se τ (SAtoms os))%I.
+  Program Definition ser_interp : semantic_type -n> semantic_type :=
+    λne T se sv,
+      (∃ os, ⌜sv = SWords (flat_map serialize_atom os)⌝ ∗ T se (SAtoms os))%I.
+  Next Obligation. solve_proper. Qed.
+  Next Obligation. solve_proper. Qed.
+  Next Obligation. solve_proper. Qed.
 
-  Definition plug_interp (se : semantic_env) (ρ : representation) : SVR :=
-    λne sv, (∃ ιs, ⌜eval_rep se ρ = Some ιs⌝ ∗ ⌜has_areps ιs sv⌝)%I.
+  Program Definition plug_interp : leibnizO representation -n> semantic_type :=
+    λne ρ se sv, (∃ ιs, ⌜eval_rep_se se ρ = Some ιs⌝ ∗ ⌜has_areps ιs sv⌝)%I.
+  Next Obligation. solve_proper. Qed.
+  Next Obligation. Admitted.
+  Next Obligation. solve_proper. Qed.
 
-  Definition span_interp (se : semantic_env) (σ : size) : SVR :=
-    λne sv, (∃ ws n, ⌜sv = SWords ws⌝ ∗ ⌜eval_size se σ = Some n⌝ ∗ ⌜length ws = n⌝)%I.
+  Program Definition span_interp : leibnizO size -n> semantic_type :=
+    λne σ se sv, (∃ ws n, ⌜sv = SWords ws⌝ ∗ ⌜eval_size se σ = Some n⌝ ∗ ⌜length ws = n⌝)%I.
+  Next Obligation. solve_proper. Qed.
+  Next Obligation. Admitted.
+  Next Obligation. solve_proper. Qed.
 
-  Definition rec_interp (vrel : value_relation) (se : semantic_env) (κ : kind) (τ : type) : SVR :=
-    λne sv,
-      match eval_kind se κ with
-      | Some sκ =>
-          let T := λne sv, ▷ vrel se (RecT κ τ) sv in
-          vrel (senv_insert_type sκ T se) τ sv
-      | None => False
-      end%I.
+  Program Definition skind_rec_interp1 sκ : semantic_type -n> semantic_env -n> SVR -n> SVR :=
+    (λne T se T0 sv, ▷ T (senv_insert_type sκ T0 se) sv)%I.
+  Next Obligation. solve_proper. Qed.
+  Next Obligation. Admitted.
+  Next Obligation. Admitted.
+  Next Obligation. Admitted.
 
-  Definition exists_mem_interp (vrel : value_relation) (se : semantic_env) (τ : type) : SVR :=
-    λne sv, (∃ μ, ▷ vrel (senv_insert_mem μ se) τ sv)%I.
-
-  Definition exists_rep_interp (vrel : value_relation) (se : semantic_env) (τ : type) : SVR :=
-    λne sv, (∃ ιs, ▷ vrel (senv_insert_rep ιs se) τ sv)%I.
-
-  Definition exists_size_interp (vrel : value_relation) (se : semantic_env) (τ : type) : SVR :=
-    λne sv, (∃ n, ▷ vrel (senv_insert_size n se) τ sv)%I.
-
-  Definition exists_type_interp
-    (vrel : value_relation) (se : semantic_env) (κ : kind) (τ : type) : SVR :=
-    λne sv,
-      (∃ sκ T,
-         ⌜eval_kind se κ = Some sκ⌝ ∗
-           ⌜stype_in_skind T sκ⌝ ∗
-           ▷ vrel (senv_insert_type sκ T se) τ sv)%I.
-
-  Program Definition type_interp0 : value_relation -n> semantic_env -n> leibnizO type -n> SVR :=
-    λne vrel se τ,
-      match τ with
-      | VarT t => type_var_interp se t
-      | I31T _ => i31_interp
-      | NumT _ nt => num_interp nt
-      | SumT (VALTYPE (SumR ρs) _) τs => sum_interp vrel se ρs τs
-      | SumT _ _ => λne _, False
-      | VariantT _ τs => variant_interp vrel se τs
-      | ProdT _ τs => prod_interp vrel se τs
-      | StructT _ τs => struct_interp vrel se τs
-      | RefT _ μ τ => ref_interp vrel se μ τ
-      | RefT _ (BaseM MemMM) τ => ref_mm_interp vrel se τ
-      | RefT _ (BaseM MemGC) τ => ref_gc_interp vrel se τ
-      | CodeRefT _ ϕ => coderef_interp vrel se ϕ
-      | SerT _ τ => ser_interp vrel se τ
-      | PlugT _ ρ => plug_interp se ρ
-      | SpanT _ σ => span_interp se σ
-      | RecT κ τ => rec_interp vrel se κ τ
-      | ExistsMemT _ τ => exists_mem_interp vrel se τ
-      | ExistsRepT _ τ => exists_rep_interp vrel se τ
-      | ExistsSizeT _ τ => exists_size_interp vrel se τ
-      | ExistsTypeT _ κ τ => exists_type_interp vrel se κ τ
-      end%I.
-  Next Obligation.
-
-  Program Definition value_se_interp0 : value_relation -n> semantic_env -n> leibnizO type -n> SVR :=
-    λne vrel se τ sv,
-      (∃ sκ, ⌜type_skind se τ = Some sκ⌝ ∗ ⌜svalue_in_skind sv sκ⌝ ∗ type_interp0 vrel se τ sv)%I.
-
-  (* TODO *)
-  Local Instance NonExpansive_value_se_interp0 (vrel : value_relation) :
-    NonExpansive (λ se, λne τ sv, value_se_interp0 vrel se τ sv).
+  Instance skind_rec_interp1_contractive sκ T se : Contractive (skind_rec_interp1 sκ T se).
   Proof.
+    unfold semantic_type in *.
+    repeat intros ?.
     cbn.
-    intros .
-    destruct τ.
-    - solve_proper.
-    repeat intros ?; cbn; try solve_proper.
+    eapply later_contractive.
+    eapply (ne_dist_later (λ svr, T (senv_insert_type sκ svr se) x0)); [|done].
+    repeat intros ?; cbn.
+    eapply (ofe_mor_ne _ _ T).
+    admit.
+  Admitted.
+
+  Program Definition skind_rec_interp sκ : semantic_type -n> semantic_type :=
+    λne T se, fixpoint (skind_rec_interp1 sκ T se).
+  Next Obligation.
+    repeat intros ?.
+    f_equiv.
+    eapply @fixpoint_ne.
+    intros.
+    by eapply (ofe_mor_ne _ _ (skind_rec_interp1 sκ T)).
+  Qed.
+  Next Obligation.
+    repeat intros ?.
+    f_equiv.
+    eapply @fixpoint_ne.
     solve_proper.
-    intros k x y.
-    induction τ.
-  Admitted.
-
-  Definition value_interp0 (vrel : value_relation) : value_relation :=
-    λne se τ sv, value_se_interp0 vrel se τ sv.
-
-  (* TODO *)
-  Instance Contractive_value_interp0 : Contractive value_interp0.
-  Admitted.
-
-  Definition value_interp : semantic_env -n> leibnizO type -n> SVR := fixpoint value_interp0.
-
-  Lemma value_interp_part_eq se τ :
-    value_interp se τ ≡ value_interp0 value_interp se τ.
-  Proof using.
-    do 2 f_equiv.
-    apply fixpoint_unfold.
   Qed.
 
-  Lemma value_interp_eq se τ sv :
-    value_interp se τ sv ⊣⊢ value_interp0 value_interp se τ sv.
-  Proof.
-    do 3 f_equiv.
-    apply fixpoint_unfold.
+  Program Definition rec_interp : leibnizO kind -n> semantic_type -n> semantic_type :=
+    λne κ T se,
+      match eval_kind_se se κ with
+      | Some sκ => skind_rec_interp sκ T se
+      | None => λne _, False
+      end%I.
+  Next Obligation. solve_proper. Qed.
+  Next Obligation.
+    cbn.
+    repeat intros ?.
+    f_equiv.
+    repeat intros ?.
+    pose proof (ofe_mor_ne _ _ (eval_kind_se) n x y H κ).
+    inversion H0 as [Heq].
+    destruct (eval_kind _ _) eqn:Hx.
+    - admit.
+    - admit.
+  Admitted.
+  Next Obligation. Admitted.
+  Next Obligation. Admitted.
+
+  Program Definition values_interp1 : listO semantic_type -n> semantic_env -n> OsR :=
+    (λne τs se os,
+      ∃ oss, ⌜os = concat oss⌝ ∗ [∗ list] τ: semantic_type; os ∈ τs; oss, τ se (SAtoms os))%I.
+  Next Obligation. solve_proper. Qed.
+  Next Obligation. solve_proper. Qed.
+  Next Obligation.
+    repeat intros ?; cbn.
+    f_equiv.
+    intros oss.
+    f_equiv.
+    erewrite (big_sepL2_ne_2); [|eapply H|reflexivity|].
+    - by instantiate (1:= fun k y1 y2 => y1 x0 (SAtoms y2)).
+    - intros.
+      solve_proper.
   Qed.
 
-  Definition values_interp (se : semantic_env) : leibnizO (list type) -n> OsR :=
-    values_interp0 value_interp se.
+  Program Definition add_skind_interp : leibnizO type -n> (semantic_env -n> SVR) -n> semantic_env -n> SVR :=
+    (λne τ T se sv,
+      ∃ sκ, ⌜type_skind se τ = Some sκ⌝ ∗ ⌜svalue_in_skind sκ sv⌝ ∗ T se sv)%I.
+  Next Obligation.
+    intros.
+    repeat intros ?.
+    f_equiv.
+    repeat intros ?.
+    f_equiv.
+    f_equiv.
+    - assert (Hprop: Proper (dist n ==> dist n) (svalue_in_skind a))
+        by apply ofe_mor_ne.
+      f_equiv.
+      by eapply Hprop.
+    - by eapply ofe_mor_ne.
+  Qed.
+  Next Obligation.
+    intros.
+    repeat intros ?.
+    f_equiv.
+    repeat intros ?.
+    cbn -[type_skind svalue_in_skind].
+    f_equiv; intros ?.
+    f_equiv; [|solve_proper].
+    f_equiv.
+    by setoid_rewrite (ofe_mor_ne _ _ type_skind).
+    Unshelve.
+    exact n.
+  Qed.
+  Next Obligation.
+    solve_proper.
+  Qed.
+  Next Obligation.
+    repeat intros ?.
+    rewrite H.
+    solve_proper.
+  Qed.
 
-  Definition closure_interp (se : semantic_env) : leibnizO function_type -n> ClR :=
-    λne ϕ, closure_interp0 value_interp se ϕ.
+  Program Definition exists_mem_interp : semantic_type -n> semantic_type :=
+    (λne T se sv, ∃ μ, T (senv_insert_mem μ se) sv)%I.
+  Next Obligation. solve_proper. Qed.
+  Next Obligation. Admitted.
+  Next Obligation. solve_proper. Qed.
+
+
+  Program Definition exists_rep_interp : semantic_type -n> semantic_type :=
+    λne T se sv, (∃ ιs, T (senv_insert_rep ιs se) sv)%I.
+  Next Obligation. solve_proper. Qed.
+  Next Obligation. Admitted.
+  Next Obligation. solve_proper. Qed.
+
+  Program Definition exists_size_interp : semantic_type -n> semantic_type :=
+    λne T se sv, (∃ n, T (senv_insert_size n se) sv)%I.
+  Next Obligation. solve_proper. Qed.
+  Next Obligation. Admitted.
+  Next Obligation. solve_proper. Qed.
+
+  Program Definition exists_type_interp (κ : kind) : semantic_type -n> semantic_type :=
+    λne T se sv,
+      (∃ T' sκ,
+         ⌜eval_kind se κ = Some sκ⌝ ∗
+         ⌜stype_in_skind T' sκ⌝ ∗
+         T (senv_insert_type sκ T' se) sv)%I.
+  Next Obligation. solve_proper. Qed.
+  Next Obligation. Admitted.
+  Next Obligation. solve_proper. Qed.
+
+  Program Definition mono_closure_interp (τs1 τs2 : list type) (Ts1 Ts2 : listO semantic_type) : semantic_env -n> ClR :=
+    λne se cl,
+      match cl with
+      | FC_func_native inst (Tf ts1 ts2) tlocs es =>
+          ⌜translate_types se τs1 = Some ts1⌝ ∗
+          ⌜translate_types se τs2 = Some ts2⌝ ∗
+          □ ▷ ∀ vs1 os1 θ,
+              atoms_interp os1 vs1 -∗
+              values_interp1 Ts1 se os1 -∗
+             rt_token rti sr θ -∗
+             na_own logrel_nais ⊤ -∗
+             ↪[frame] Build_frame (vs1 ++ n_zeros tlocs) inst -∗
+             ↪[RUN] -∗
+             let Φ vs2 :=
+               (∃ os2, atoms_interp os2 vs2 ∗
+                       values_interp1 Ts2 se os2) ∗
+                 (∃ θ', rt_token rti sr θ') ∗ na_own logrel_nais ⊤
+             in
+             CWP es UNDER [(length ts2, const Φ)]; Some (length ts2, Φ) {{ const Φ }}
+      | FC_func_host _ _ => False
+      end%I.
+  Next Obligation. Admitted.
+  Next Obligation. Admitted.
+
+  Program Definition forall_mem_interp : (semantic_env -n> ClR) -n> (semantic_env -n> ClR) :=
+    (λne FT se cl, ∀ μ, FT (senv_insert_mem μ se) cl)%I.
+  Next Obligation. solve_proper. Qed.
+  Next Obligation. Admitted.
+  Final Obligation. solve_proper. Qed.
+
+  Program Definition forall_rep_interp : (semantic_env -n> ClR) -n> (semantic_env -n> ClR) :=
+    (λne FT se cl, ∀ ρ, FT (senv_insert_rep ρ se) cl)%I.
+  Next Obligation. solve_proper. Qed.
+  Next Obligation. Admitted.
+  Final Obligation. solve_proper. Qed.
+
+  Program Definition forall_size_interp : (semantic_env -n> ClR) -n> (semantic_env -n> ClR) :=
+    (λne FT se cl, ∀ n, FT (senv_insert_size n se) cl)%I.
+  Next Obligation. solve_proper. Qed.
+  Next Obligation. Admitted.
+  Final Obligation. solve_proper. Qed.
+
+  Program Definition forall_type_interp κ : (semantic_env -n> ClR) -n> (semantic_env -n> ClR) :=
+    (λne FT se cl, ∃ sκ,
+        ⌜eval_kind se κ = Some sκ⌝ ∗
+        ∀ sκ_T T,
+          ⌜subskind_of sκ_T sκ⌝ -∗
+          ⌜stype_in_skind T sκ_T⌝ -∗
+          FT (senv_insert_type sκ_T T se) cl)%I.
+  Next Obligation. solve_proper. Qed.
+  Next Obligation. Admitted.
+  Final Obligation. solve_proper. Qed.
+
+  Fixpoint type_interp (τ : leibnizO type) : semantic_env -n> SVR :=
+    match τ with
+    | VarT t => type_var_interp t
+    | I31T _ => i31_interp
+    | NumT _ nt => num_interp nt
+    | SumT κ τs => sum_interp κ (map type_interp τs)
+    | VariantT _ τs => variant_interp (map type_interp τs)
+    | ProdT _ τs => prod_interp (map type_interp τs)
+    | StructT _ τs => struct_interp (map type_interp τs)
+    | RefT _ μ τ => ref_interp μ (type_interp τ)
+    | SerT _ τ => ser_interp (type_interp τ)
+    | PlugT _ ρ => plug_interp ρ
+    | SpanT _ σ => span_interp σ
+    | RecT κ τ => rec_interp κ (type_interp τ)
+    | ExistsMemT _ τ => exists_mem_interp (type_interp τ)
+    | ExistsRepT _ τ => exists_rep_interp (type_interp τ)
+    | ExistsSizeT _ τ => exists_size_interp (type_interp τ)
+    | ExistsTypeT _ κ τ => exists_type_interp κ (type_interp τ)
+    | CodeRefT _ ϕ => coderef_interp (closure_interp ϕ)
+    end%I
+  with closure_interp (ϕ : function_type) : semantic_env -n> ClR :=
+    match ϕ with
+    | MonoFunT τs1 τs2 => mono_closure_interp τs1 τs2 (map type_interp τs1) (map type_interp τs2)
+    | ForallMemT ϕ' => forall_mem_interp (closure_interp ϕ')
+    | ForallRepT ϕ' => forall_rep_interp (closure_interp ϕ')
+    | ForallSizeT ϕ' => forall_size_interp (closure_interp ϕ')
+    | ForallTypeT κ ϕ' => forall_type_interp κ (closure_interp ϕ')
+    end%I.
+
+  Program Definition value_interp : semantic_env -n> leibnizO type -n> SVR := λne se τ, type_interp τ se.
+  Next Obligation. solve_proper. Qed.
+  Next Obligation. solve_proper. Qed.
+
+  Program Definition values_interp : semantic_env -n> leibnizO (list type) -n> OsR :=
+    λne se τs,
+      values_interp1 (map type_interp τs) se.
+  Next Obligation. solve_proper. Qed.
+  Next Obligation. solve_proper. Qed.
 
   Definition locals_interp (se : semantic_env) :
     leibnizO local_ctx -n> leibnizO (list (list atom)) -n> iPropO Σ :=
     λne L oss, ([∗ list] τ; os ∈ L; oss, value_interp se τ (SAtoms os))%I.
 
-  Definition frame_interp (se : semantic_env) :
+  Program Definition frame_interp (se : semantic_env) :
     leibnizO (list (list primitive)) -n>
       leibnizO local_ctx -n>
       leibnizO wlocal_ctx -n>
@@ -833,7 +873,7 @@ Section instr.
     [∗ list] i ↦ ϕ ∈ M.(mc_functions),
       ∃ i' cl,
         ⌜inst.(inst_funcs) !! (funcimm mr.(mr_func_user) + i)%nat = Some i'⌝ ∗
-          closure_interp senv_empty ϕ cl ∗
+          closure_interp ϕ senv_empty cl ∗
           na_inv logrel_nais (ns_fun (N.of_nat i')) (N.of_nat i' ↦[wf] cl).
 
   Definition table_entry_interp (off : nat) (i : nat) (ϕ : function_type) : iProp Σ :=
@@ -841,7 +881,7 @@ Section instr.
       ⌜N_nat_repr (off + i) nt⌝ ∗
         ⌜N_Z_repr nt zt⌝ ∗
         ⌜zt < Wasm_int.Int32.modulus⌝%Z ∗
-        closure_interp senv_empty ϕ cl ∗
+        closure_interp ϕ senv_empty cl ∗
         na_inv logrel_nais (ns_tab nt) (N.of_nat sr.(sr_table) ↦[wt][nt] Some i') ∗
         na_inv logrel_nais (ns_fun (N.of_nat i')) (N.of_nat i' ↦[wf] cl).
 
@@ -864,8 +904,9 @@ Section instr.
 
   Global Instance Persistent_instance_interp mr M WT inst : Persistent (instance_interp mr M WT inst).
   Proof.
-    typeclasses eauto.
-  Defined.
+    unfold instance_interp.
+    (* typeclasses eauto. *)
+  Admitted.
 
   Definition mask_locs_eq (lmask : nat -> Prop) (fr fr' : frame) : Prop :=
     forall i, lmask i -> fr.(f_locs) !! i = fr'.(f_locs) !! i.
@@ -996,7 +1037,7 @@ Section module.
           ∃ bs j cl,
             N.of_nat i ↪[vis] datatypes.Build_module_export bs (MED_func j) ∗
               N.of_nat (funcimm j) ↦[wf] cl ∗
-              closure_interp rti sr senv_empty ϕ cl ∗
+              closure_interp rti sr ϕ senv_empty cl ∗
               ⌜imports !! (funcimm mr.(mr_func_user) + i)%nat = Some (N.of_nat (funcimm j))⌝) -∗
        ([∗ list] i ↦ '_ ∈ ω.(mt_exports),
           ∃ bs j,
@@ -1008,7 +1049,7 @@ Section module.
                i ↪[mods] m ∗
                ([∗ list] i ↦ ϕ ∈ ω.(mt_exports),
                  ∃ j cl, (* TODO: same j as precond *)
-                   N.of_nat (funcimm j) ↦[wf] cl ∗ closure_interp rti sr senv_empty ϕ cl) }})%I.
+                   N.of_nat (funcimm j) ↦[wf] cl ∗ closure_interp rti sr ϕ senv_empty cl) }})%I.
 
   (* TODO *)
   Definition has_module_type_sem (m : W.module) (ω : module_type) : iProp Σ :=
